src/Inject.v
@@ -1,0 +1,150 @@
+Require Import compcert.lib.Coqlib.
+Require Import compcert.lib.Maps.
+Require Import compcert.lib.Integers.
+
+Require Import compcert.common.AST.
+Require Import compcert.common.Values.
+Require Import compcert.common.Globalenvs.
+Require Import compcert.common.Memory.
+Require Import compcert.common.Events.
+Require Import compcert.common.Switch.
+
+Require Import TraceSemantics.
+
+Require Import compcert.backend.Cminor.
+Require Import HighValues.
+
+Require Import StructTact.StructTactics.
+Require Import StructTact.Util.
+
+Require Import EricTact.
+
+Require Import Cmajor.
+
+Section GENV.
+
+  Variable ge : Genv.t Cminor.fundef unit.
+
+Lemma inject_unop :
+  forall op arg arg' res m,
+    global_blocks_valid ge m ->
+    eval_unop op arg = Some res ->
+    Val.inject (Mem.flat_inj (Mem.nextblock m)) arg arg' ->
+    exists res',
+      eval_unop op arg' = Some res' /\ Val.inject (Mem.flat_inj (Mem.nextblock m)) res res'.
+Proof.
+  intros.
+  destruct op; simpl in *; try find_inversion;
+    try solve [eexists; split; eauto;
+               match goal with
+               | [ |- Val.inject _ (?X _ arg) (?X _ arg') ] => unfold X; inv H1; simpl; try econstructor; eauto
+               | [ |- Val.inject _ (?X arg) (?X arg') ] => unfold X; inv H1; simpl; try econstructor; eauto
+               end];
+
+    try solve [inv H1; simpl in *; try congruence;
+               try unfold option_map in *;
+               try break_match_hyp; try congruence; find_inversion; solve [eauto]].
+Qed.
+
+
+Lemma inject_cmpu :
+  forall m m',
+    Mem.inject (Mem.flat_inj (Mem.nextblock m)) m m' ->
+    forall a b c,
+      Val.inject (Mem.flat_inj (Mem.nextblock m)) (Val.cmpu (Mem.valid_pointer m) c a b) (Val.cmpu (Mem.valid_pointer m') c a b).
+Proof.
+  intros.
+  assert (Hvp : forall b ofs, Mem.valid_pointer m b ofs = true -> Mem.valid_pointer m' b ofs = true). {
+    intros.
+    eapply Mem.valid_pointer_inject in H0; try eassumption.
+    erewrite Z.add_0_r in H0. eassumption.
+    unfold Mem.flat_inj.
+    unfold Mem.valid_pointer in *.
+    unfold Mem.perm_dec in *.
+    unfold Mem.perm_order'_dec in *.
+    unfold proj_sumbool in *.
+    break_match_hyp; try congruence.
+    unfold Mem.perm_order' in *.
+    break_match_hyp; try solve [inv p].
+    break_match; try reflexivity.
+    eapply Mem.nextblock_noaccess in n.
+    erewrite n in Heqo. congruence.
+  } idtac.
+  
+  destruct c eqn:?; unfold Val.cmpu; unfold Val.cmpu_bool; simpl;
+    repeat (break_match; try congruence; simpl);
+    try solve [try econstructor; eauto];
+    repeat 
+      (try rewrite andb_true_iff in *;
+       try rewrite andb_false_iff in *;
+       try rewrite orb_false_iff in *;
+       try rewrite orb_true_iff in *);
+       repeat progress (try break_or; try break_and);
+       try congruence;
+       match goal with
+       | [ H : Mem.valid_pointer m ?X ?Y = true, H2 : Mem.valid_pointer m' ?X ?Y = false |- _ ] => eapply Hvp in H; congruence
+       end.
+Qed.
+
+Lemma inject_binop :
+  forall op a a' b b' res m m',
+    eval_binop op a b m = Some res ->
+    Val.inject (Mem.flat_inj (Mem.nextblock m)) a a' ->
+    Val.inject (Mem.flat_inj (Mem.nextblock m)) b b' ->
+    Mem.inject (Mem.flat_inj (Mem.nextblock m)) m m' ->
+    exists res',
+      eval_binop op a' b' m' = Some res' /\ Val.inject (Mem.flat_inj (Mem.nextblock m)) res res'.
+Proof.
+    intros.
+    destruct op; inv H0; inv H1; simpl in H; inv H;
+    try solve [
+          try destruct a'; try destruct b';
+          simpl in H; inv H;
+          eexists; split;
+            match goal with
+            | [ |- Val.inject (Mem.flat_inj (Mem.nextblock m)) _ _ ] => idtac
+            | [ |- _ ] => simpl; try reflexivity
+            end;
+            eauto];
+
+    try solve [eexists; split; simpl; try reflexivity;
+               eapply inject_cmpu; eauto];
+
+    try solve [
+          unfold Mem.flat_inj in *;
+          repeat (break_match_hyp; try congruence);
+          repeat match goal with
+                 | [ H : Some _ = Some _ |- _ ] => invc H
+                 end;
+          try destruct a'; try destruct b';
+          try simpl in H; try inv H;
+          eexists; split;
+          match goal with
+          | [ |- Val.inject (Mem.flat_inj (Mem.nextblock m)) _ _ ] => idtac
+          | [ |- _ ] => simpl; try reflexivity
+          end;
+          eauto;
+          try econstructor; eauto;
+          try break_match; try congruence; try reflexivity;
+          repeat rewrite Int.add_zero; try reflexivity;
+          try econstructor; eauto;
+          try destruct c; try unfold Val.cmp;
+          try unfold Val.cmpf;
+          try unfold Val.cmpfs;
+          try unfold Val.cmplu;
+          try unfold Val.cmpl;
+          simpl;
+          try break_match; try unfold Vtrue; try unfold Vfalse;
+          try econstructor; eauto;
+          try eapply inject_cmpu; eauto
+        ].
+
+    eexists; split; simpl; try reflexivity.
+    destruct c; unfold Val.cmpl; simpl; unfold Val.of_bool;
+      break_match; try unfold Vtrue; try unfold Vfalse; try econstructor; eauto.
+    eexists; split; simpl; try reflexivity.
+    destruct c; unfold Val.cmplu; simpl; unfold Val.of_bool;
+      break_match; try unfold Vtrue; try unfold Vfalse; try econstructor; eauto.
+Qed.
+
+End GENV.
